src/Ex/Mesi/Mesi.v
@@ -382,8 +382,7 @@ Section System.
         rule.rqu[2~>0]
         :me oidx
         :requires
-           (fun ost mins =>
-              ost#[dir].(dir_st) = mesiI /\ mesiNP < ost#[status] < mesiM)
+           (fun ost mins => mesiNP < ost#[status] < mesiM)
         :transition
            (ost --> {| miv_id := mesiInvRq; miv_value := O |}).
 
@@ -399,8 +398,7 @@ Section System.
         rule.rqu[2~>1]
         :me oidx
         :requires
-           (fun ost mins =>
-              ost#[dir].(dir_st) = mesiI /\ mesiNP < ost#[status])
+           (fun ost mins => mesiNP < ost#[status])
         :transition
            (ost --> {| miv_id := mesiInvWRq; miv_value := ost#[val] |}).
 
